proofs of assumption (actually eassumption)

theories/InstantiateI.v
@@ -1,5 +1,6 @@
 Require Import ExtLib.Data.HList.
 Require Import MirrorCore.ExprI.
+Require Import MirrorCore.CtxLogic.
 
 Section definitions.
   Variables typ expr : Type.
@@ -9,6 +10,16 @@ Section definitions.
 
   (** instantiate **)
   Variable instantiate : (nat -> option expr) -> nat -> expr -> expr.
+
+  Definition sem_preserves_if_ho tus tvs
+             (P : exprT tus tvs Prop -> Prop)
+             (f : nat -> option expr) : Prop :=
+    forall u e t get,
+      f u = Some e ->
+      nth_error_get_hlist_nth _ tus u = Some (@existT _ _ t get) ->
+      exists eD,
+        exprD' tus tvs e t = Some eD /\
+        P (fun us vs => get us = eD us vs).
 
   Definition sem_preserves_if tus tvs
              (P : hlist _ tus -> hlist _ tvs -> Prop)
@@ -40,6 +51,41 @@ Section definitions.
         forall us vs vs',
           P us vs ->
           eD us (hlist_app vs' vs) = eD' us (hlist_app vs' vs).
+
+  Definition sem_instantiate_ho {T TD} (R : TD -> TD -> Prop)
+             (exprD' : forall tus tvs, T -> option (exprT tus tvs TD))
+             (instantiate : (nat -> option expr) -> nat -> T -> T)
+  : Prop :=
+    forall tus tvs f e tvs' eD P (App : ExprTApplicative P),
+      sem_preserves_if_ho tus tvs P f ->
+      exprD' tus (tvs' ++ tvs) e = Some eD ->
+      exists eD',
+        exprD' tus (tvs' ++ tvs) (instantiate f (length tvs') e) = Some eD' /\
+        P (fun us vs => forall vs',
+                          eD us (hlist_app vs' vs) = eD' us (hlist_app vs' vs)).
+
+(*
+  Goal (forall t : typ, @sem_instantiate_ho expr (typD t) (@eq _)
+                                            (fun tus tvs e => exprD' tus tvs e t)
+                                            instantiate) ->
+  exprD'_instantiate.
+  Proof.
+    unfold exprD'_instantiate, sem_instantiate_ho.
+    intuition.
+    specialize (@H t tus tvs f e tvs' eD
+                   (fun (P' : exprT tus tvs Prop) => forall us vs,
+                                P us vs ->
+                                P' us vs)).
+    destruct H.
+    - clear. constructor; firstorder.
+    - red. red in H0. intros.
+      eapply H0 in H; eauto.
+    - eauto.
+    - exists x. intuition.
+  Qed.
+*)
+
 End definitions.
 
 Arguments sem_preserves_if {typ expr RType Expr} _ _ _ _ : rename.
+Arguments sem_preserves_if_ho {typ expr RType Expr} tus tvs C f : rename.
